Refactor probe, beta, and test as star rel_step (slow)'

src/Codes.v
@@ -8,6 +8,8 @@ Require Import Coq.Classes.RelationClasses.
 Require Import Coq.Classes.Morphisms.
 Require Export Notations.
 
+(** ** Codes *)
+
 Inductive code {Var : Set} : Set :=
   | code_var : Var -> code
   | code_ap : code -> code -> code
@@ -44,36 +46,55 @@ Notation "x (+) y" := (code_r * x * y) : code_scope.
 
 Definition code_join {Var : Set} x y : Code Var := x || y.
 
-Inductive probe {Var : Set} : Code Var -> Code Var -> Prop :=
-  | probe_refl {x} : probe x x
-  | probe_trans {x} y {z} : probe x y -> probe y z -> probe x z
-  | probe_top {x y} : probe x y -> probe x (y * TOP).
+(** ** Reduction relations *)
 
-Inductive beta {Var : Set} : Code Var -> Code Var -> Prop :=
-  | beta_refl {x} : beta x x
-  | beta_trans {x} y {z} : beta x y -> beta y z -> beta x z
-  | beta_ap_left {x x' y} : beta x x' -> beta (x * y) (x' * y)
-  | beta_ap_right {x y y'} : beta y y' -> beta (x * y) (x * y')
-  | beta_i {x} : beta (I * x) x
-  | beta_k {x y} : beta (K * x * y) x
-  | beta_b {x y z} : beta (B * x * y * z) (x * (y * z))
-  | beta_c {x y z} : beta (C * x * y * z) (x * z * y)
-  | beta_s {x y z} : beta (S * x * y * z) (x * z * (y * z))
-  | beta_j_ap {x y z} : beta ((x || y) * z) (x * z || y * z)
-  | beta_r_ap {x y z} : beta ((x (+) y) * z) (x * z (+) y * z)
-  | beta_r_idem {x} : beta (x (+) x) x
-  | beta_r_sym {x y} : beta (x (+) y) (y (+) x)
-  | beta_r_sym_sym {w x y z} : beta ((w(+)x) (+) (y(+)z)) ((x(+)y) (+) (z(+)w)).
+Inductive star {Var : Set} (r : relation (Code Var)) : relation (Code Var) :=
+  | star_step {x y} : r x y -> star r x y
+  | star_refl {x} : star r x x
+  | star_trans {x} y {z} : star r x y -> star r y z -> star r x z.
+Hint Constructors star.
 
-Inductive test {Var : Set} : Code Var -> Code Var -> Prop :=
-  | test_refl {x} : test x x
-  | test_trans {x} y {z} : test x y -> test y z -> test x z
-  | test_ap_left {x x' y} : test x x' -> test (x * y) (x' * y)
-  | test_ap_right {x y y'} : test y y' -> test (x * y) (x * y')
-  | test_top x : test (TOP * x) TOP
-  | test_bot x : test x BOT
-  | test_j_left {x y} : test (x || y) x
-  | test_j_right {x y} : test (x || y) y.
+Inductive astar {Var : Set} (r : relation (Code Var)) : relation (Code Var) :=
+  | astar_step {x y} : r x y -> astar r x y
+  | astar_refl {x} : astar r x x
+  | astar_trans {x} y {z} : astar r x y -> astar r y z -> astar r x z
+  | astar_left {x x' y} : astar r x x' -> astar r (x * y) (x' * y)
+  | astar_right {x y y'} : astar r y y' -> astar r (x * y) (x * y').
+Hint Constructors astar.
+
+Inductive probe_step {Var : Set} : Code Var -> Code Var -> Prop :=
+  | probe_top {x y} : probe_step x y -> probe_step x (y * TOP).
+Hint Constructors probe_step.
+
+Definition probe {Var : Set} : relation (Code Var) := star probe_step.
+Hint Unfold probe.
+
+Inductive beta_step {Var : Set} : Code Var -> Code Var -> Prop :=
+  | beta_i {x} : beta_step (I * x) x
+  | beta_k {x y} : beta_step (K * x * y) x
+  | beta_b {x y z} : beta_step (B * x * y * z) (x * (y * z))
+  | beta_c {x y z} : beta_step (C * x * y * z) (x * z * y)
+  | beta_s {x y z} : beta_step (S * x * y * z) (x * z * (y * z))
+  | beta_j_ap {x y z} : beta_step ((x || y) * z) (x * z || y * z)
+  | beta_r_ap {x y z} : beta_step ((x (+) y) * z) (x * z (+) y * z)
+  | beta_r_idem {x} : beta_step (x (+) x) x
+  | beta_r_sym {x y} : beta_step (x (+) y) (y (+) x)
+  | beta_r_sym_sym {w x y z} :
+      beta_step ((w(+)x) (+) (y(+)z)) ((x(+)y) (+) (z(+)w)).
+Hint Constructors beta_step.
+
+Definition beta {Var : Set} : relation (Code Var) := astar beta_step.
+Hint Unfold beta.
+
+Inductive test_step {Var : Set} : Code Var -> Code Var -> Prop :=
+  | test_top x : test_step (TOP * x) TOP
+  | test_bot x : test_step x BOT
+  | test_j_left {x y} : test_step (x || y) x
+  | test_j_right {x y} : test_step (x || y) y.
+Hint Constructors test_step.
+
+Definition test {Var : Set} : relation (Code Var) := astar test_step.
+Hint Unfold test.
 
 Definition conv {Var : Set} (x : Code Var) : Prop :=
   exists y z, probe x y /\ beta y z /\ test z TOP.
@@ -82,27 +103,14 @@ Inductive prob {Var : Set} : Code Var -> Prop :=
   | prob_top : prob TOP
   | prob_bot : prob BOT
   | prob_r p q : prob p -> prob q -> prob (p (+) q).
+Hint Constructors prob.
 
 Definition pconv {Var : Set} (x p : Code Var) : Prop :=
   prob p /\ exists y z, probe x y /\ beta y z /\ test z p.
 
-Hint Constructors probe.
-Hint Constructors beta.
-Hint Constructors test.
-Hint Constructors prob.
-
-Definition Beta_i (Var : Set) := (@beta_i Var).
-Definition Beta_k (Var : Set) := (@beta_k Var).
-Definition Beta_b (Var : Set) := (@beta_b Var).
-Definition Beta_c (Var : Set) := (@beta_c Var).
-Definition Beta_s (Var : Set) := (@beta_s Var).
-Definition Beta_j_ap (Var : Set) := (@beta_j_ap Var).
-Definition Beta_r_ap (Var : Set) := (@beta_r_ap Var).
-Definition Beta_r_idem (Var : Set) := (@beta_r_idem Var).
-
-Hint Rewrite Beta_i Beta_k Beta_b Beta_c Beta_j_ap Beta_r_ap Beta_r_idem
+Hint Rewrite @beta_i @beta_k @beta_b @beta_c @beta_j_ap @beta_r_ap @beta_r_idem
   : beta_safe.
-Hint Rewrite Beta_s : beta_unsafe.
+Hint Rewrite @beta_s : beta_unsafe.
 
 Tactic Notation "beta_simpl" :=
   timeout 10
@@ -150,13 +158,17 @@ Proof. auto. Qed.
 
 Instance probe_transitive (Var : Set) : Transitive (@probe Var).
 Proof.
-  intros x y z; apply probe_trans.
+  intros x y z; apply star_trans.
 Qed.
 
 Instance probe_preorder (Var : Set) : PreOrder (@probe Var).
 Proof.
   split; [apply probe_reflexive | apply probe_transitive].
 Qed.
+
+Instance probe_subrelation (Var : Set) :
+  @subrelation (Code Var) probe_step probe.
+Proof. simpl_relation. Qed.
 
 Instance probe_confluent (Var : Set) :
   Commuting (flip (@probe Var)) (@probe Var).
@@ -170,13 +182,17 @@ Proof. auto. Qed.
 
 Instance beta_transitive (Var : Set) : Transitive (@beta Var).
 Proof.
-  intros x y z; apply beta_trans.
+  intros x y z; apply astar_trans.
 Qed.
 
 Instance beta_preorder (Var : Set) : PreOrder (@beta Var).
 Proof.
   split; [apply beta_reflexive | apply beta_transitive].
 Qed.
+
+Instance beta_subrelation (Var : Set) :
+  @subrelation (Code Var) beta_step beta.
+Proof. simpl_relation. Qed.
 
 Instance code_ap_beta (Var : Set) :
   Proper (beta ==> beta ==> beta) (@code_ap Var).
@@ -193,7 +209,7 @@ Admitted.
 
 Instance test_transitive (Var : Set) : Transitive (@test Var).
 Proof.
-  intros x y z Hxy Hyz; apply test_trans with y; auto.
+  intros x y z Hxy Hyz; apply astar_trans with y; auto.
 Qed.
 
 Instance test_reflexive (Var : Set) : Reflexive (@test Var).
@@ -203,6 +219,10 @@ Instance test_preorder (Var : Set) : PreOrder (@test Var).
 Proof.
   split; [apply test_reflexive | apply test_transitive].
 Qed.
+
+Instance test_subrelation (Var : Set) :
+  @subrelation (Code Var) test_step test.
+Proof. simpl_relation. Qed.
 
 Instance code_ap_test (Var : Set) : Proper (test ++> test ++> test) (@code_ap Var).
 Proof.
