src/TypeConstructor.v
@@ -275,26 +275,26 @@ Proof.
   induction H; auto.
   - transitivity y; auto.
   - rewrite code_eq_y; beta_simpl.
-    rewrite test_j_left.
-    rewrite test_j_left.
-    rewrite test_j_left.
+    rewrite (astar_step _ test_j_left).
+    rewrite (astar_step _ test_j_left).
+    rewrite (astar_step _ test_j_left).
     auto.
   - rewrite code_eq_y; beta_simpl.
-    rewrite test_j_left.
-    rewrite test_j_left.
-    rewrite test_j_right.
+    rewrite (astar_step _ test_j_left).
+    rewrite (astar_step _ test_j_left).
+    rewrite (astar_step _ test_j_right).
     auto.
   - rewrite code_eq_y; beta_simpl.
-    rewrite test_j_left.
-    rewrite test_j_right.
+    rewrite (astar_step _ test_j_left).
+    rewrite (astar_step _ test_j_right).
     auto.
   - rewrite code_eq_y; beta_simpl.
-    rewrite test_j_right.
-    rewrite test_j_left.
+    rewrite (astar_step _ test_j_right).
+    rewrite (astar_step _ test_j_left).
     rewrite IHA_above; auto.
   - rewrite code_eq_y; beta_simpl.
-    rewrite test_j_right.
-    rewrite test_j_right.
+    rewrite (astar_step _ test_j_right).
+    rewrite (astar_step _ test_j_right).
     rewrite IHA_above; auto.
 Qed.
 
